theories/cancellation/CancelGetTid.v
@@ -1,0 +1,30 @@
+Require Import CRIS.
+Require Import LMod LModTr GSim GSimFacts GSimTactics.
+Require Import MInline MInlineIntro MInlineElim ElimRel.
+
+Lemma cancel_gettid `{_crisG: !crisG Γ Σ α β τ _S _I, _concG: !concG} md sp :
+  CANCEL_GOAL md sp NativeGetTidE HoareGetTidE.
+Proof.
+  r; i. subst.
+  ziter_l; ziter_r. rewrite x0 x1 /=. zstep_l.
+  zstep_r. zstep_r. ziter_l. zstep_l.
+  ziter_r. zstep_r. ziter_r. zstep_r. ired.
+  ziter_r. zstep_r. zstep_r. ziter_r. zstep_r. zstep_r.
+  ziter_r. zstep_r. ziter_r. zstep_r. ziter_r. zstep_r.
+  ziter_r. zstep_r. ziter_r. zstep_r.
+  ziter_r. zstep_r. ired. ziter_r. zstep_r. exists r_t. zstep_r.
+  ziter_r. zstep_r. unshelve eexists.
+  { des; split; eauto.
+    { eapply Own_wand_valid with (a1 := r_s); eauto. rewrite RS.
+      iIntros ">[_ [$ _]]"; eauto. }
+    rewrite x5. iIntros ">[$ $]". iPureIntro. sym.
+    eapply Own_pure_soundness with (a:=r_s); eauto.
+    iIntros "S". iPoseProof (RS with "S") as ">[_ [T [TA _]]]".
+    iPoseProof (x5 with "T") as ">[T _]".
+    iApply (TidToken_agree with "[T]"); iFrame.
+  }
+  ired. zstep_r. ziter_r. zstep_r. ziter_r. zstep_r. ziter_r. zstep_r.
+  eapply KEY with (r_diff:=ε); eauto.
+  { rewrite length_insert list_insert_id //. }
+  { econs; eauto. eapply KTR. }
+(*SLOW*)Qed.
