theories/cancellation/CancelYield.v
@@ -1,0 +1,35 @@
+Require Import CRIS.
+Require Import LMod LModTr GSim GSimFacts GSimTactics.
+Require Import MInline MInlineIntro MInlineElim ElimRel.
+
+Lemma cancel_yield `{_crisG: !crisG Γ Σ α β τ _S _I, _concG: !concG} md sp tid :
+  CANCEL_GOAL md sp (NativeYieldE tid) (HoareYieldE tid).
+Proof.
+  r; i. subst.
+  ziter_l; ziter_r. rewrite x0 x1 /=. zstep_l.
+  zstep_r. zstep_r. ziter_r. zstep_r. ziter_r. zstep_r. ired.
+  ziter_r. zstep_r. zstep_r. ziter_r. zstep_r. ziter_r. zstep_r. zstep_r.
+  ziter_r. zstep_r. ziter_r. zstep_r. ziter_r. zstep_r.
+
+  destruct (decide (tid < length rs_diff)); cycle 1.
+  {
+    ziter_l. destruct (<[cid:=_]> srcs !! tid) eqn:FIND.
+    { eapply lookup_lt_Some in FIND. rewrite length_insert in FIND. nia. }
+    { zstep_l. zstep_l. }
+  }
+  destruct (decide (tid = cid)); subst.
+  {
+    ziter_l. zstep_l. ziter_r. zstep_r. ziter_r. zstep_r. ired.
+    ziter_r. zstep_r. exists r_t. zstep_r. ziter_r. zstep_r. unshelve eexists; ired.
+    { admit. }
+    zstep_r. ziter_r. zstep_r. ziter_r. zstep_r. ziter_r. zstep_r.
+    eapply KEY with (r_diff:=ε); eauto.
+    { rewrite length_insert list_insert_id //. }
+    { eapply thread_rel_body; eauto. eapply KTR. }
+  }
+  { do 2 dup l. rename l into SRC, l0 into TGT, l1 into RES.
+    rewrite EQLEN2 in SRC. rewrite EQLEN2 EQLEN in TGT.
+    Search (_ < length _ → _ !! _ = Some _).
+    eapply lookup_lt_Some
+  }
+Admitted.
